h2k: just got a Bluespec L1 cache module!

syn/ex/Mesi/MesiComp.v
@@ -14,10 +14,15 @@ Section Tests.
   Definition ostin: string := "ost".
 
   Definition KMesi: Kind := Bit 3.
+  Definition mesiM {var}: Expr var (SyntaxKind KMesi) := ($3)%kami_expr.
+  Definition mesiE {var}: Expr var (SyntaxKind KMesi) := ($2)%kami_expr.
+  Definition mesiS {var}: Expr var (SyntaxKind KMesi) := ($1)%kami_expr.
+  Definition mesiI {var}: Expr var (SyntaxKind KMesi) := ($0)%kami_expr.
+  
   Definition KDir :=
     STRUCT { "dir_st" :: KMesi;
-             "dir_excl" :: KIdxQ;
-             "dir_sharers" :: Array KIdxQ (Nat.pow 2 hcfg_children_max_lg) }.
+             "dir_excl" :: KIdxO;
+             "dir_sharers" :: Array KIdxO (S hcfg_children_max) }.
 
   Instance MesiCompExtType: CompExtType :=
     {| kind_of_hetype :=
@@ -26,17 +31,56 @@ Section Tests.
                     end
     |}.
 
+  Fixpoint compile_dir_exp
+           (var: Kind -> Type) {het}
+           (ostvars: HVector.hvec (Vector.map (fun hty => var (kind_of hty)) hostf_ty))
+           (he: heexp (hvar_of var) het): Expr var (SyntaxKind (kind_of het)) :=
+    (match he in (hexp_dir _ h) return (Expr var (SyntaxKind (kind_of h))) with
+     | HDirC _ => #(HVector.hvec_ith ostvars (Fin.FS (Fin.FS (Fin.FS Fin.F1))))
+     | HDirGetSt dir => ((compile_dir_exp ostvars dir)!KDir@."dir_st")
+     | HDirGetExcl dir => ((compile_dir_exp ostvars dir)!KDir@."dir_excl")
+     | HDirGetStO oidx dir => TODO _
+     | HDirGetSh dir => ((compile_dir_exp ostvars dir)!KDir@."dir_sharers")
+     | HDirAddSharer oidx dir => TODO _
+     | HDirRemoveSharer oidx dir => TODO _
+     | HDirSetM oidx => (STRUCT { "dir_st" ::= mesiM;
+                                  "dir_excl" ::= compile_bexp ostvars oidx;
+                                  "dir_sharers" ::= $$Default })
+     | HDirSetE oidx => (STRUCT { "dir_st" ::= mesiE;
+                                  "dir_excl" ::= compile_bexp ostvars oidx;
+                                  "dir_sharers" ::= $$Default })
+     | HDirSetS oinds => TODO _
+     | HDirSetI _ => (STRUCT { "dir_st" ::= mesiI;
+                               "dir_excl" ::= $$Default;
+                               "dir_sharers" ::= $$Default })
+     | HRqUpFrom oidx => TODO _
+     | HRsUpFrom oidx => TODO _
+     | HDownTo oidx => TODO _
+     | HRqUpFromM oinds => TODO _
+     | HRsUpFromM oinds => TODO _
+     | HDownToM oinds => TODO _
+     | HSingleton se => TODO _
+     end)%kami_expr.
+
   Instance MesiCompExtExp: CompExtExp :=
-    {| compile_eexp :=
-         fun var het ostVars he =>
-           match he in (hexp_dir _ h) return (kind_of h) @ (var) with
-           | HDirC _ =>
-             #(HVector.hvec_ith ostVars (Fin.FS (Fin.FS (Fin.FS Fin.F1))))
-           | _ => TODO _
-           end%kami_expr
-    |}.
+    {| compile_eexp := compile_dir_exp |}.
 
   (* Opaque icons'. *)
   Existing Instance MesiHOStateIfcFull.
+
+  Definition hrule: HRule (Mesi.l1InvRqUpUp oidx).
+  Proof.
+    ⇑rule.
+  Defined.
+  Definition crule :=
+    Eval vm_compute in (compile_Rule oidx uln dln ostin (existT _ _ hrule)).
+  
+  Definition okl1 :=
+    Eval vm_compute in (compile_Object (existT _ _ (hl1 oidx))).
+  Definition kl1: Modules :=
+    Eval simpl in (match okl1 with
+                   | Some m => m
+                   | None => Mod nil nil nil
+                   end).
 
 End Tests.
