syn/ex/Mesi/MesiExt.v
@@ -1,0 +1,18 @@
+(** TODO: better to have a file in Kami that "exports" such modules *)
+Require Import Kami.Synthesize.
+Require Import Kami.Ext.BSyntax.
+Require Import ExtrOcamlBasic ExtrOcamlNatInt ExtrOcamlString.
+Extraction Language OCaml.
+
+Set Extraction Optimize.
+Set Extraction KeepSingleton.
+Unset Extraction AutoInline.
+
+Require Import MesiComp.
+
+Definition targetM: Kami.Syntax.Modules := kl1.
+Definition targetS := getModuleS targetM.
+Definition targetB := ModulesSToBModules targetS.
+
+(* Extraction "./Target.ml" targetB. *)
+
